src/dafny/core/precompiled.dfy
@@ -33,7 +33,15 @@ module Precompiled {
         // (1) ECDSA Recover
         (data,v,r,s)=>(data),
         // (2) SHA256
-        data=>(data)
+        data=>data,
+        // (3) RIPEMD160
+        data=>data,
+        // (4) ModExp
+        (B,E,M)=>([]),
+        // (9) Blake2f
+        data=>data,
+        // Sha3
+        data=>0
     )
 
     // The type for an external ECDSA recover implementation, where we have v, r
@@ -41,11 +49,19 @@ module Precompiled {
     type EcdsaRecoverFn = (Array<u8>, u8, u256, u256)->Array<u8>
     // The type for an external Sha256 implementation.
     type Sha256Fn = Array<u8> -> Array<u8>
+    // The type for an external RipEmd160 implementation.
+    type RipEmd160Fn = Array<u8> -> Array<u8>
+    // The type for an external ModExp implementation.
+    type ModExpFn = (Array<u8>,Array<u8>,Array<u8>)->Array<u8>
+    // The type for an external Blake2f implementation.
+    type Blake2Fn = Array<u8> -> Array<u8>
+    // The type for an external Sha3 implementation.
+    type Sha3Fn = Array<u8> -> u256
 
     // Define the type of the precompiled dispatch function.  This accepts an
     // address and an array of input data, and returns either nothing (in the
     // event of a failure) or an array of output data and a gas cost.
-    datatype Dispatcher = Dispatcher(ecdsa: EcdsaRecoverFn, sha256: Sha256Fn) {
+    datatype Dispatcher = Dispatcher(ecdsa: EcdsaRecoverFn, sha256: Sha256Fn, ripemd160: RipEmd160Fn, modexp: ModExpFn, blake2f: Blake2Fn, sha3: Sha3Fn) {
         // Call a precompiled contract.  This function is marked opaque to
         // ensure that, when verifying against this function, no assumptions are
         // made about the possible return values.
@@ -53,18 +69,18 @@ module Precompiled {
             match address
             case 1 => CallEcdsaRecover(ecdsa,data)
             case 2 => CallSha256(sha256,data)
-            // case 3 => CallRipEmd160(data)
-            // case 4 => CallID(data)
-            // case 5 => CallModExp(data)
+            case 3 => CallRipEmd160(ripemd160,data)
+            case 4 => CallID(data)
+            case 5 => CallModExp(modexp,data)
             // case 6 => CallBnAdd(data)
             // case 7 => CallBnMul(data)
             // case 8 => CallSnarkV(data)
-            // case 9 => CallBlake2f(data)
+            case 9 => CallBlake2f(blake2f,data)
             case _ => None
         }
 
         function {:opaque} Sha3(data: Array<u8>) : u256 {
-            0 // FOR NOW
+            sha3(data)
         }
     }
 
@@ -122,9 +138,8 @@ module Precompiled {
     /**
      * RipEmd160
      */
-    function CallRipEmd160(data: Array<u8>) : Option<(Array<u8>,nat)> {
-        //Some((External.ripEmd160(data), CostRipEmd160(data)))
-        None
+    function CallRipEmd160(fn: RipEmd160Fn, data: Array<u8>) : Option<(Array<u8>,nat)> {
+        Some((fn(data), CostRipEmd160(data)))
     }
 
     /**
@@ -168,7 +183,7 @@ module Precompiled {
      * we compue B^E % M.  All words are unsigned integers in big endian format.
      * See also EIP-2565.
      */
-    function CallModExp(data: Array<u8>) : Option<(Array<u8>,nat)> {
+    function CallModExp(fn: ModExpFn, data: Array<u8>) : Option<(Array<u8>,nat)> {
         // Length of B
         var lB := Bytes.ReadUint256(data,0) as nat;
         // Length of E
@@ -181,15 +196,14 @@ module Precompiled {
         var E := Bytes.Slice(data,96+lB,lE);
         // Extract M(odulo)
         var M := Bytes.Slice(data,96+lB+lE,lM);
-        // // Compute modexp
-        // var modexp := External.modExp(B,E,M);
-        // // Compute lEp
-        // var lEp := LenEp(lB,E,data);
-        // // Gas calculation
-        // var gascost := Int.Max(200, (f(Int.Max(lM,lB)) * Int.Max(lEp,1)) / G_QUADDIVISOR);
-        // // Done
-        // Some((modexp,gascost))
-        None
+        // Compute modexp
+        var modexp := fn(B,E,M);
+        // Compute lEp
+        var lEp := LenEp(lB,E,data);
+        // Gas calculation
+        var gascost := Int.Max(200, (f(Int.Max(lM,lB)) * Int.Max(lEp,1)) / G_QUADDIVISOR);
+        // Done
+        Some((modexp,gascost))
     }
 
     /**
@@ -257,14 +271,13 @@ module Precompiled {
     // (9) Blake2f
     // ========================================================================
 
-    function CallBlake2f(data: Array<u8>) : Option<(Array<u8>,nat)> {
-        // if |data| == 213 && data[212] in {0,1}
-        // then
-        //     var r := U32.Read(data,0) as nat;
-        //     // FIXME: pull out stuff!
-        //     Some((External.blake2f(data),r))
-        // else
-        //     None
-        None
+    function CallBlake2f(fn: Blake2Fn,data: Array<u8>) : Option<(Array<u8>,nat)> {
+        if |data| == 213 && data[212] in {0,1}
+        then
+            var r := U32.Read(data,0) as nat;
+            // FIXME: pull out stuff!
+            Some((fn(data),r))
+        else
+            None
     }
 }
