src/dafny/evmstate.dfy
@@ -66,6 +66,7 @@ module EvmState {
      */
     datatype Raw = EVM(
         context: Context.T,
+        precompiled: Precompiled.Dispatcher,
         world : WorldState.T,
         stack   : Stack.Stack,
         memory  : Memory.T,
@@ -79,6 +80,7 @@ module EvmState {
     // requirements.  This should not be consider as a valid or useful instance
     // of the EVM though.
     const EVM_WITNESS : Raw := EVM(Context.DEFAULT,
+            Precompiled.DEFAULT,
             WorldState.Create(map[0:=WorldState.DefaultAccount()]),
             Stack.Create(),
             Memory.Create(),
@@ -363,7 +365,7 @@ module EvmState {
         requires !evm.world.Exists(address)
         requires |code| <= Code.MAX_CODE_SIZE {
             // Compute code hash
-            var hash := evm.context.precompiled.Sha3(code);
+            var hash := evm.precompiled.Sha3(code);
             // Create account
             var data := WorldState.CreateAccount(nonce,balance,Storage.Create(storage),Code.Create(code),hash);
             // Done
@@ -635,7 +637,7 @@ module EvmState {
      * @param depth The current call depth.
      * @param opcode The opcode causing this call.
      */
-    function Call(world: WorldState.T, ctx: Context.T, substate: SubState.T, codeAddress: u160, value: u256, gas: nat, depth: nat) : State
+    function Call(world: WorldState.T, ctx: Context.T, precompiled: Precompiled.Dispatcher, substate: SubState.T, codeAddress: u160, value: u256, gas: nat, depth: nat) : State
     // Sender account must exist
     requires world.Exists(ctx.sender)  {
         // Address of called contract
@@ -656,7 +658,7 @@ module EvmState {
                 if codeAddress >= 1 && codeAddress <= 9
                 then
                     // Call precompiled contract
-                    match ctx.precompiled.Call(codeAddress,ctx.callData)
+                    match precompiled.Call(codeAddress,ctx.callData)
                     case None => ERROR(INVALID_PRECONDITION,0,[])
                     case Some((data,gascost)) => if gas >= gascost
                         then RETURNS(gas - gascost, data, nw, substate)
@@ -670,7 +672,7 @@ module EvmState {
                         // Construct fresh EVM
                         var stack := Stack.Create();
                         var mem := Memory.Create();
-                        var evm := EVM(ctx,nw,stack,mem,cod,substate,gas,0);
+                        var evm := EVM(ctx,precompiled,nw,stack,mem,cod,substate,gas,0);
                         // Off we go!
                         EXECUTING(evm)
     }
@@ -684,7 +686,7 @@ module EvmState {
      * @param gas The available gas to use for the call.
      * @param depth The current call depth.
      */
-    function Create(world: WorldState.T, ctx: Context.T, substate: SubState.T, initcode: seq<u8>, gas: nat, depth: nat) : State
+    function Create(world: WorldState.T, ctx: Context.T, precompiled: Precompiled.Dispatcher, substate: SubState.T, initcode: seq<u8>, gas: nat, depth: nat) : State
     requires |initcode| <= Code.MAX_CODE_SIZE
     requires world.Exists(ctx.sender) {
         var endowment := ctx.callValue;
@@ -709,7 +711,7 @@ module EvmState {
                 var cod := Code.Create(initcode);
                 // Mark new account as having been accessed
                 var ss := substate.AccountAccessed(ctx.address);
-                var evm := EVM(ctx,nw,stack,mem,cod,ss,gas,0);
+                var evm := EVM(ctx,precompiled,nw,stack,mem,cod,ss,gas,0);
                 // Off we go!
                 EXECUTING(evm)
     }
@@ -751,11 +753,11 @@ module EvmState {
             var origin := evm.context.origin;
             var gasPrice := evm.context.gasPrice;
             var block := evm.context.block;
-            var precompiled := evm.context.precompiled;
+            var precompiled := evm.precompiled;
             // Construct new context
-            var ctx := Context.Create(sender,origin,recipient,delegateValue,callData,writePermission,gasPrice,block,precompiled);
+            var ctx := Context.Create(sender,origin,recipient,delegateValue,callData,writePermission,gasPrice,block);
             // Make the call!
-            Call(evm.world,ctx,evm.substate,code,callValue,gas,depth+1)
+            Call(evm.world,ctx,precompiled,evm.substate,code,callValue,gas,depth+1)
         }
 
         /**
@@ -804,11 +806,11 @@ module EvmState {
             var origin := evm.context.origin;
             var gasPrice := evm.context.gasPrice;
             var block := evm.context.block;
-            var precompiled := evm.context.precompiled;
+            var precompiled := evm.precompiled;
             // Construct new context
-            var ctx := Context.Create(sender,origin,address,endowment,[],evm.context.writePermission,gasPrice,block,precompiled);
+            var ctx := Context.Create(sender,origin,address,endowment,[],evm.context.writePermission,gasPrice,block);
             // Make the creation!
-            Create(evm.world,ctx,evm.substate,initcode,gas,depth+1)
+            Create(evm.world,ctx,precompiled,evm.substate,initcode,gas,depth+1)
         }
 
         /**
@@ -846,7 +848,7 @@ module EvmState {
                     else if vm.gas < depositcost then st.Push(0)
                     else
                         // Compute code hash
-                        var hash := evm.context.precompiled.Sha3(vm.data);
+                        var hash := evm.precompiled.Sha3(vm.data);
                         // Initialise contract code for new account
                         var nworld := vm.world.SetCode(address,vm.data,hash);
                         // Mark account as having been accessed
